disk-betree/BetreeRefinement.dfy
@@ -5,8 +5,10 @@ include "BetreeInv.dfy"
 module BetreeRefinement {
   import opened DBI = BetreeInv
   import opened G = BetreeGraph
+  import opened BetreeSpec`Internal
 
   type Lookup = DB.Lookup
+  type UIOp = DB.MS.UI.Op<Value>
     
   datatype LookupResult = LookupResult(lookup: Lookup, result: Value)
   
@@ -123,17 +125,18 @@ module BetreeRefinement {
     }
   }
 
-  lemma QueryStepRefinesMap(k: DB.Constants, s: DB.Variables, s': DB.Variables, key: Key, value: Value, lookup: Lookup)
+  lemma QueryStepRefinesMap(k: DB.Constants, s: DB.Variables, s': DB.Variables, uiop: UIOp, key: Key, value: Value, lookup: Lookup)
     requires Inv(k, s)
-    requires DB.Query(k, s, s', key, value, lookup)
+    requires DB.Query(k, s, s', uiop, key, value, lookup)
     requires Inv(k, s')
-    ensures DB.MS.Next(Ik(k), I(k, s), I(k, s'))
+    ensures DB.MS.Next(Ik(k), I(k, s), I(k, s'), uiop)
   
-  lemma InsertMessageStepRefinesMap(k: DB.Constants, s: DB.Variables, s': DB.Variables, key: Key, msg: BufferEntry, oldroot: Node)
+  lemma InsertMessageStepRefinesMap(k: DB.Constants, s: DB.Variables, s': DB.Variables, uiop: UIOp, key: Key, msg: BufferEntry, oldroot: Node)
     requires Inv(k, s)
+    requires BetreeStepUI(BetreeInsert(MessageInsertion(key, msg, oldroot)), uiop)
     requires DBI.InsertMessage(k.bck, s.bcv, s'.bcv, key, msg, oldroot)
     requires Inv(k, s')
-    ensures DB.MS.Next(Ik(k), I(k, s), I(k, s'))
+    ensures DB.MS.Next(Ik(k), I(k, s), I(k, s'), uiop)
   {
     var value := msg.value;
 
@@ -142,91 +145,95 @@ module BetreeRefinement {
     assert EquivalentLookupsWithPut(k, s, s', key, value);
     
     EquivalentLookupsWithPutImplInterpsPut(k, s, s', key, value);
-    assert DB.MS.NextStep(Ik(k), I(k, s), I(k, s'), DB.MS.WriteStep(key, value));
+    assert DB.MS.NextStep(Ik(k), I(k, s), I(k, s'), uiop, DB.MS.WriteStep(key, value));
   }
 
-  lemma FlushStepRefinesMap(k: DB.Constants, s: DB.Variables, s': DB.Variables,
+  lemma FlushStepRefinesMap(k: DB.Constants, s: DB.Variables, s': DB.Variables, uiop: UIOp,
                                            parentref: Reference, parent: Node, childref: Reference, child: Node, newchildref: Reference, movedKeys: iset<Key>)
     requires Inv(k, s)
+    requires uiop.NoOp?
     requires DBI.Flush(k.bck, s.bcv, s'.bcv, parentref, parent, childref, child, newchildref, movedKeys)
     requires Inv(k, s')
-    ensures DB.MS.NextStep(Ik(k), I(k, s), I(k, s'), DB.MS.StutterStep)
+    ensures DB.MS.NextStep(Ik(k), I(k, s), I(k, s'), uiop, DB.MS.StutterStep)
   {
     FlushEquivalentLookups(k, s, s', parentref, parent, childref, child, newchildref, movedKeys);
     EquivalentLookupsImplInterpsEqual(k, s, s');
     assert I(k, s) == I(k, s');
   }
 
-  lemma GrowStepRefinesMap(k: DB.Constants, s: DB.Variables, s': DB.Variables, oldroot: Node, newchildref: Reference)
+  lemma GrowStepRefinesMap(k: DB.Constants, s: DB.Variables, s': DB.Variables, uiop: UIOp, oldroot: Node, newchildref: Reference)
     requires Inv(k, s)
+    requires uiop.NoOp?
     requires DBI.Grow(k.bck, s.bcv, s'.bcv, oldroot, newchildref)
     requires Inv(k, s')
-    ensures DB.MS.NextStep(Ik(k), I(k, s), I(k, s'), DB.MS.StutterStep)
+    ensures DB.MS.NextStep(Ik(k), I(k, s), I(k, s'), uiop, DB.MS.StutterStep)
   {
     GrowEquivalentLookups(k, s, s', oldroot, newchildref);
     EquivalentLookupsImplInterpsEqual(k, s, s');
     assert I(k, s) == I(k, s');
   }
 
-  lemma SplitStepRefinesMap(k: DB.Constants, s: DB.Variables, s': DB.Variables, fusion: DB.BetreeSpec.NodeFusion)
+  lemma SplitStepRefinesMap(k: DB.Constants, s: DB.Variables, s': DB.Variables, uiop: UIOp, fusion: DB.BetreeSpec.NodeFusion)
     requires Inv(k, s)
+    requires uiop.NoOp?
     requires DBI.Split(k.bck, s.bcv, s'.bcv, fusion)
     requires Inv(k, s')
-    ensures DB.MS.NextStep(Ik(k), I(k, s), I(k, s'), DB.MS.StutterStep)
+    ensures DB.MS.NextStep(Ik(k), I(k, s), I(k, s'), uiop, DB.MS.StutterStep)
   {
     SplitEquivalentLookups(k, s, s', fusion);
     EquivalentLookupsImplInterpsEqual(k, s, s');
     assert I(k, s) == I(k, s');
   }
 
-  lemma BetreeStepRefinesMap(k: DB.Constants, s: DB.Variables, s':DB.Variables, betreeStep: DBI.BetreeSpec.BetreeStep)
+  lemma BetreeStepRefinesMap(k: DB.Constants, s: DB.Variables, s':DB.Variables, uiop: UIOp, betreeStep: DBI.BetreeSpec.BetreeStep)
     requires Inv(k, s)
-    requires DB.NextStep(k, s, s', DB.BetreeStep(betreeStep))
+    requires BetreeStepUI(betreeStep, uiop)
+    requires DB.NextStep(k, s, s', uiop, DB.BetreeStep(betreeStep))
     ensures Inv(k, s')
-    ensures DB.MS.Next(Ik(k), I(k, s), I(k, s'))
+    ensures DB.MS.Next(Ik(k), I(k, s), I(k, s'), uiop)
   {
-    NextPreservesInv(k, s, s');
+    NextPreservesInv(k, s, s', uiop);
     match betreeStep {
-      case BetreeInsert(ins) => InsertMessageStepRefinesMap(k, s, s', ins.key, ins.msg, ins.oldroot);
-      case BetreeFlush(flush) => FlushStepRefinesMap(k, s, s', flush.parentref, flush.parent, flush.childref, flush.child, flush.newchildref, flush.movedKeys);
-      case BetreeGrow(growth) => GrowStepRefinesMap(k, s, s', growth.oldroot, growth.newchildref);
-      case BetreeSplit(fusion) => SplitStepRefinesMap(k, s, s', fusion);
+      case BetreeInsert(ins) => InsertMessageStepRefinesMap(k, s, s', uiop, ins.key, ins.msg, ins.oldroot);
+      case BetreeFlush(flush) => FlushStepRefinesMap(k, s, s', uiop, flush.parentref, flush.parent, flush.childref, flush.child, flush.newchildref, flush.movedKeys);
+      case BetreeGrow(growth) => GrowStepRefinesMap(k, s, s', uiop, growth.oldroot, growth.newchildref);
+      case BetreeSplit(fusion) => SplitStepRefinesMap(k, s, s', uiop, fusion);
     }
   }
 
-  lemma GCStepRefinesMap(k: DB.Constants, s: DB.Variables, s':DB.Variables, refs: iset<DB.BI.Reference>)
+  lemma GCStepRefinesMap(k: DB.Constants, s: DB.Variables, s':DB.Variables, uiop: UIOp, refs: iset<DB.BI.Reference>)
     requires Inv(k, s)
-    requires DB.NextStep(k, s, s', DB.GCStep(refs))
+    requires DB.NextStep(k, s, s', uiop, DB.GCStep(refs))
     requires Inv(k, s')
-    ensures DB.MS.NextStep(Ik(k), I(k, s), I(k, s'), DB.MS.StutterStep)
+    ensures DB.MS.NextStep(Ik(k), I(k, s), I(k, s'), uiop, DB.MS.StutterStep)
   {
     GCStepEquivalentLookups(k, s, s', refs);
     EquivalentLookupsImplInterpsEqual(k, s, s');
     assert I(k, s) == I(k, s');
   }
 
-  lemma BetreeRefinesMapNextStep(k: DB.Constants, s: DB.Variables, s':DB.Variables, step: DB.Step)
+  lemma BetreeRefinesMapNextStep(k: DB.Constants, s: DB.Variables, s':DB.Variables, uiop: UIOp, step: DB.Step)
     requires Inv(k, s)
-    requires DB.NextStep(k, s, s', step)
+    requires DB.NextStep(k, s, s', uiop, step)
     ensures Inv(k, s')
-    ensures DB.MS.Next(Ik(k), I(k, s), I(k, s'))
+    ensures DB.MS.Next(Ik(k), I(k, s), I(k, s'), uiop)
   {
-    NextPreservesInv(k, s, s');
+    NextPreservesInv(k, s, s', uiop);
     match step {
-      case QueryStep(key, value, lookup) => QueryStepRefinesMap(k, s, s', key, value, lookup);
-      case BetreeStep(betreeStep) => BetreeStepRefinesMap(k, s, s', betreeStep);
-      case GCStep(refs) => GCStepRefinesMap(k, s, s', refs);
+      case QueryStep(key, value, lookup) => QueryStepRefinesMap(k, s, s', uiop, key, value, lookup);
+      case BetreeStep(betreeStep) => BetreeStepRefinesMap(k, s, s', uiop, betreeStep);
+      case GCStep(refs) => GCStepRefinesMap(k, s, s', uiop, refs);
     }
   }
     
-  lemma BetreeRefinesMapNext(k: DB.Constants, s: DB.Variables, s':DB.Variables)
+  lemma BetreeRefinesMapNext(k: DB.Constants, s: DB.Variables, s':DB.Variables, uiop: UIOp)
     requires Inv(k, s)
-    requires DB.Next(k, s, s')
+    requires DB.Next(k, s, s', uiop)
     ensures Inv(k, s')
-    ensures DB.MS.Next(Ik(k), I(k, s), I(k, s'))
+    ensures DB.MS.Next(Ik(k), I(k, s), I(k, s'), uiop)
   {
-    NextPreservesInv(k, s, s');
-    var step :| DB.NextStep(k, s, s', step);
-    BetreeRefinesMapNextStep(k, s, s', step);
+    NextPreservesInv(k, s, s', uiop);
+    var step :| DB.NextStep(k, s, s', uiop, step);
+    BetreeRefinesMapNextStep(k, s, s', uiop, step);
   }
 }
